online: repair extract message and state types

examples/Online/DY.Online.Data.fst
@@ -11,21 +11,19 @@ open DY.Lib
 ///
 /// (They are the same as for the simple 2 message protocol)
 
-
-
 (*** Message Type ***)
 
 /// for each of the two messages we define an abstract message type
 
 [@@ with_bytes bytes] // ignore this line for now
 type ping_t = {
-  p_alice: principal;
-  p_n_a : bytes;
+  alice: principal;
+  n_a : bytes;
 }
 
 [@@ with_bytes bytes] // ignore this line for now
-type ack = {
-  a_n_a : bytes;
+type ack_t = {
+  n_a : bytes;
 }
 
 /// the overall abstract message type
@@ -33,9 +31,9 @@ type ack = {
 /// and using the above abstract types for each of them)
 
 [@@ with_bytes bytes] // ignore this line for now
-type message =
-  | Ping: (ping:ping_t) -> message
-  | Ack: (ack:ack) -> message
+type message_t =
+  | Ping: (ping:ping_t) -> message_t
+  | Ack: (ack:ack_t) -> message_t
 
 
 /// We use Comparse to generate the corresponding message formats.
@@ -46,12 +44,15 @@ type message =
 /// We are not going into the details of how Comparse works.
 
 
-/// We let Comparse generate a parser `ps_ping` for the abstract `ping` type
+/// We let Comparse generate a parser `ps_ping_t` for the abstract `ping_t` type
+
 %splice [ps_ping_t] (gen_parser (`ping_t))
 
-%splice [ps_ack] (gen_parser (`ack))
+/// ... and the same for the other abstract message types
 
-%splice [ps_message] (gen_parser (`message))
+%splice [ps_ack_t] (gen_parser (`ack_t))
+
+%splice [ps_message_t] (gen_parser (`message_t))
 
 /// With the above parsers, we can make our `message` type an instance of
 /// Comparse's `parseable_serializeable` class.
@@ -59,7 +60,8 @@ type message =
 /// but this is the step that enables us to call
 /// `parse message buff` and `serialize message msg`
 /// to translate between bytes and our abstract message type.
-instance parseable_serializeable_bytes_message: parseable_serializeable bytes message = mk_parseable_serializeable ps_message
+
+instance parseable_serializeable_bytes_message_t: parseable_serializeable bytes message_t = mk_parseable_serializeable ps_message_t
 
 
 (*** State Type ***)
@@ -68,49 +70,51 @@ instance parseable_serializeable_bytes_message: parseable_serializeable bytes me
 /// for the three states stored by Alice and Bob after each step of the protocol.
 
 [@@ with_bytes bytes]
-type sent_ping = {
-  sp_bob : principal;
-  sp_n_a : bytes;
+type sent_ping_t = {
+  bob : principal;
+  n_a : bytes;
 }
 
 [@@ with_bytes bytes]
-type sent_ack = {
-  sa_alice: principal;
-  sa_n_a : bytes;
+type sent_ack_t = {
+  alice: principal;
+  n_a : bytes;
 }
 
 [@@ with_bytes bytes]
-type received_ack = {
-  ra_bob : principal;
-  ra_n_a : bytes;
+type received_ack_t = {
+  bob : principal;
+  n_a : bytes;
 }
 
 [@@ with_bytes bytes]
-type state = 
-  | SentPing: (ping:sent_ping) -> state
-  | SentAck: (ack:sent_ack) -> state
-  | ReceivedAck: (rack:received_ack) -> state
+type state_t = 
+  | SentPing: (ping:sent_ping_t) -> state_t
+  | SentAck: (ack:sent_ack_t) -> state_t
+  | ReceivedAck: (rack:received_ack_t) -> state_t
 
 /// As for messages, we use Comparse to generate
-/// a parser and serializer for our abstract state type.
+/// a parser and serializer for our abstract state types.
 
-%splice [ps_sent_ping] (gen_parser (`sent_ping))
-%splice [ps_sent_ack] (gen_parser (`sent_ack))
-%splice [ps_received_ack] (gen_parser (`received_ack))
-%splice [ps_state] (gen_parser (`state))
+%splice [ps_sent_ping_t] (gen_parser (`sent_ping_t))
+%splice [ps_sent_ack_t] (gen_parser (`sent_ack_t))
+%splice [ps_received_ack_t] (gen_parser (`received_ack_t))
+%splice [ps_state_t] (gen_parser (`state_t))
 
 /// Now, we can call
 /// `parse state buff` and `serialize state st`
 /// to translate between bytes and the abstract state type.
-instance parseable_serializeable_bytes_state: parseable_serializeable bytes state = mk_parseable_serializeable ps_state
+
+instance parseable_serializeable_bytes_state_t: parseable_serializeable bytes state_t = mk_parseable_serializeable ps_state_t
 
 /// We tag our protocol level states,
 /// so that they are distinguishable from any internal DY* states. 
 
-instance local_state_state: local_state state = {
+instance local_state_state: local_state state_t = {
   tag = "P.State";
-  format = parseable_serializeable_bytes_state;
+  format = parseable_serializeable_bytes_state_t;
 }
+
 
 
 (*** PKI ***)
